tools/Vale/src/emit_common_quick_code.fs
@@ -1,0 +1,63 @@
+// Implement '{:quick}' procedures
+
+module Emit_common_quick_code
+
+open Ast
+open Ast_util
+open Parse
+open Parse_util
+open Transform
+open Emit_common_base
+open Microsoft.FSharp.Math
+open System.Numerics
+
+let build_qcode (env:env) (loc:loc) (p:proc_decl):decls =
+  (*
+  [@"opaque_to_smt"]
+  let va_qcode_Add3 () : quickCode unit (va_code_Add3 ()) = qblock (
+    QSeq (va_quick_Add64 (OReg Rax) (OConst 1)) (
+    QSeq (va_quick_Add64 (OReg Rax) (OConst 1)) (
+    QSeq (va_quick_Add64 (OReg Rax) (OConst 1)) (
+    QEmpty ()
+    )))
+  )
+  *)
+  let fParams = [] in
+  let tRetQuick = TApp (TName (Id "quickCode"), []) in
+  let eQuick = EApply (Id "QEmpty", []) in
+  let fCodes =
+    {
+      fname = Reserved ("qcode_" + (string_of_id p.pname));
+      fghost = NotGhost;
+      fargs = fParams;
+      fret = tRetQuick;
+      fbody = Some eQuick;
+      fattrs = [(Id "opaque_to_smt", [])];
+    }
+    in
+  [(loc, DFun fCodes)]
+
+let build_proc_body (env:env) (loc:loc) (p:proc_decl) (code:exp) (ens:exp):stmt list =
+  let makeArg (x, t, storage, io, attrs) = EVar x
+  let args = List.map makeArg p.pargs in
+  // let (sM, fM, g) = wpSound_X code (qCodes_X ARGS) s0 (fun s0 sM gs -> let (g1, ..., gn) = g in ENS) in
+  // let (g1, ..., gn) = g in
+  let s0 = Reserved "s0" in
+  let fM = Reserved "fM" in
+  let sM = Reserved "sM" in
+  let g = Reserved "g" in
+  let wpSound_X = Reserved ("wpSound_" + (string_of_id p.pname)) in
+  let qCodes_X = Reserved ("qcode_" + (string_of_id p.pname)) in
+  let ghostRets = List.collect (fun (x, t, g, _, _) -> match g with XGhost -> [(x, t)] | _ -> []) p.prets in
+  let gAssigns = List.map (fun (x, _) -> (x, None)) ghostRets in
+  let letGs = EBind (BindLet, [EVar g], gAssigns, [], ens) in
+  let funCont = EBind (Lambda, [], [(s0, None); (sM, None); (g, None)], [], letGs) in
+  let eWpSound = EApply (wpSound_X, [code; EApply (qCodes_X, args); EVar s0; funCont]) in
+  let sWpSound = SAssign ([(sM, None); (fM, None); (g, None)], eWpSound) in
+  let gAssigns = List.map (fun (x, _) -> (x, None)) ghostRets in
+  let sAssignGs =
+    match ghostRets with
+    | [] -> []
+    | _ -> [SAssign (gAssigns, EVar g)]
+    in
+  [sWpSound] @ sAssignGs
