tools/Vale/src/emit_common_quick_export.fs
@@ -25,32 +25,41 @@ Example: Add64
   UPDATES_SM = (update_operand dst (eval_operand dst sM) ({s0 with flags = sM.flags}))
 
 // Function
-let wp_X PARAMS (s0:state) (wpContinue:state -> A -> Type0) : Type0 =
+let wp_X PARAMS (s0:state) (k:state -> A -> Type0) : Type0 =
   REQ(s0) /\
   (forall MODS GHOSTRETS.
     let sM = UPDATES(s0, MODS) in
     ENS(s0, sM) ==>
-    wpContinue sM (g1, ..., gn)
+    k sM (g1, ..., gn)
   )
 
 // Procedure
-val wpProof_X PARAMS (aN:Type0) (qs:state -> state * fuel * aN -> Type0) (s0:state) (wpContinue:(state -> A -> Type0)) :
-  Ghost (sM:state & f0:fuel & g:A & va_quickProc_q aN (qs sM) True (va_quickProc_q aN (qs sM) (wpContinue sM g) unit))
-  (requires wp_X ARGS s0 wpContinue)
-  (ensures fun (|sM, f0, _, _|) -> eval_code (va_code_X ARGS) s0 f0 sM)
+val wpMonotone_X PARAMS (s0:state) (k1:state -> A -> Type0) (k2:state -> A -> Type0) : Lemma
+  (requires (forall (s:state) (g:A). k1 s g ==> k2 s g))
+  (ensures wp_X ARGS s0 k1 ==> wp_X ARGS s0 k2) =
+let wpMonotone_X s0 k1 k2 = ()
 
-let wpProof_X ARGS aN qs s0 wpContinue =
+val wpCompute_X PARAMS (s0:state) : Ghost (state * fuel * A)
+  (requires wp_X ARGS s0 k_true)
+  (ensures fun _ -> True)
+let wpCompute_X s0 =
   let (sM, f0, g1, ..., gn) = va_lemma_X (va_code_X ARGS) s0 ARGS in
   let g = (g1, ..., gn) in
+  (sM, f0, g)
+
+val wpProof_X PARAMS (s0:state) (k:state -> A -> Type0) : Lemma
+  (requires wp_X ARGS s0 k)
+  (ensures t_ensure (va_code_X ARGS) (wp_X ARGS) (wpMonotone_X ARGS) (wpCompute_X ARGS) s0 k)
+let wpProof_X s0 k =
+  let (sM, f0, g1, ..., gn) = va_lemma_X (va_code_X ARGS) s0 ARGS in
   va_lemma_upd_update sM;
   assert (state_eq sM UPDATES_SM);
-  let f : (va_quickProc_q aN (qs sM) (wpContinue sM g) unit -> Ghost (state * fuel * aN) True (qs sM)) = fun x -> x () in
-  (|sM, f0, g, f|)
+  ()
 
 // Function
 [@"opaque_to_smt"]
 let quick_X PARAMS : quickCode A (va_code_X ARGS) =
-  va_QProc (va_code_X ARGS) (wp_X ARGS) (wpProof_X ARGS)
+  va_QProc (va_code_X ARGS) (wp_X ARGS) (wpMonotone_X ARGS) (wpCompute_X ARGS) (wpProof_X ARGS)
 *)
 
 let makeFrame (env:env) (p:proc_decl) (s0:id) (sM:id):exp * formal list =
@@ -99,6 +108,7 @@ let build_proc (env:env) (loc:loc) (p:proc_decl):decls =
   let tArgsCode = List.map (fun x -> TName x) xArgsCode in
   let eArgsCode = List.map (fun x -> EVar x) xArgsCode in
   let eUnit = EApply (Id "tuple", []) in
+  let eTrue = EVar (Id "True") in
   let tType0 = TName (Id "Type0") in
   let tUnit = TName (Id "unit") in
   let tTrue = TName (Id "True") in
@@ -110,22 +120,22 @@ let build_proc (env:env) (loc:loc) (p:proc_decl):decls =
     | xts -> TApp (TName (Id "tuple"), List.map snd xts)
     in
   let wp_X = Reserved ("wp_" + (string_of_id p.pname)) in
+  let wpMonotone_X = Reserved ("wpMonotone_" + (string_of_id p.pname)) in
+  let wpCompute_X = Reserved ("wpCompute_" + (string_of_id p.pname)) in
   let wpProof_X = Reserved ("wpProof_" + (string_of_id p.pname)) in
   let lemma_X = Reserved ("lemma_" + (string_of_id p.pname)) in
-  let aN = Reserved "aN" in
-  let qs = Reserved "qs" in
+  let s = Reserved "s" in
   let s0 = Reserved "s0" in
   let sM = Reserved "sM" in
   let f0 = Reserved "f0" in
   let x = Reserved "x" in
   let g = Reserved "g" in
-  let f = Reserved "f" in
-  let pf = Reserved "pf" in
-  let quickProc_q = Reserved "quickProc_q" in
-  let wpContinue = Reserved "wpContinue" in
-  let tAN = TName aN in
+  let k = Reserved "k" in
+  let k1 = Reserved "k1" in
+  let k2 = Reserved "k2" in
+  let k_true = Id "k_true" in
   let tContinue = TApp (TName (Id "fun"), [tState; tA; tType0]) in
-  let argContinue = (wpContinue, Some tContinue) in
+  let argContinue = (k, Some tContinue) in
   let tCode = TApp (TName (Reserved ("code_" + (string_of_id p.pname))), tArgsCode) in
   let eCode = EApply (Reserved ("code_" + (string_of_id p.pname)), eArgsCode) in
 
@@ -141,7 +151,7 @@ let build_proc (env:env) (loc:loc) (p:proc_decl):decls =
   let (updatesX, wpFormals) = makeFrame env p s0 sM in
   let (wpReqs, wpEnss) = collect_specs (List.concat pspecs) in
   let (wpReq, wpEns) = (and_of_list (reqIsExps @ wpReqs), and_of_list wpEnss) in
-  let continueM = EApply (wpContinue, [EVar sM; ghostRetTuple]) in
+  let continueM = EApply (k, [EVar sM; ghostRetTuple]) in
   let ensContinue = EOp (Bop BImply, [wpEns; continueM]) in
   let letEnsContinue = EBind (BindLet, [updatesX], [(sM, None)], [], ensContinue) in
   let wpForall = EBind (Forall, [], wpFormals @ ghostRetFormals, [], letEnsContinue) in
@@ -156,57 +166,85 @@ let build_proc (env:env) (loc:loc) (p:proc_decl):decls =
       fattrs = [(Id "public", [])];
     }
     in
-  // wpProof_X declaration
-  let tRetQuick = TApp (TName (Reserved "quickCode"), [tA; tCode]) in
-  let tQsTuple = TApp (TName (Id "tuple"), [tState; tFuel; tAN]) in
-  let tQs = TApp (TName (Id "fun"), [tState; tQsTuple; tType0]) in
+
+  // wpMonotone_X declaration
+  let applyOpt f args = match args with [] -> EVar f | _ -> EApply (f, args) in
+  let appArgs x = applyOpt x eArgs in
   let arg x t = (x, t, XGhost, In, []) in
-  let pAN = arg aN tType0 in
-  let pQs = arg qs tQs in
   let pS0 = arg s0 tState in
-  let pWpContinue = arg wpContinue tContinue in
+  let pK1 = arg k1 tContinue in
+  let pK2 = arg k2 tContinue in
+  let appSG k = EApply (k, [EVar s; EVar g]) in
+  let reqImp = EOp (Bop BImply, [appSG k1; appSG k2]) in
+  let reqForall = EBind (Forall, [], [(s, Some tState); (g, Some tA)], [], reqImp) in // TODO: triggers
+  let appWp k = EApply (wp_X, eArgs @ [EVar s0; EVar k]) in
+  let ensImp = EOp (Bop BImply, [appWp k1; appWp k2]) in
+  let specReq = Requires (Unrefined, reqForall) in
+  let specEns = Ensures (Unrefined, ensImp) in
+  // wpMonotone_X body
+  let pMonotone =
+    {
+      pname = wpMonotone_X;
+      pghost = Ghost;
+      pinline = Outline;
+      pargs = pargs @ [pS0; pK1; pK2];
+      prets = [];
+      pspecs = [(loc, specReq); (loc, specEns)];
+      pbody = Some [];
+      pattrs = [];
+    }
+    in
+
+  // wpCompute_X declaration
   let rSM = arg sM tState in
   let rF0 = arg f0 tFuel in
   let rG = arg g tA in
-  let tQ = TApp (TName qs, [TName sM]) in
-  let tWpContinue = TApp (TName wpContinue, [TName sM; TName g]) in
-  let tPf1 = TApp (TName quickProc_q, [tAN; tQ; tWpContinue; tUnit]) in
-  let tPf2 = TApp (TName quickProc_q, [tAN; tQ; tTrue; tPf1]) in
-  let rPf = arg pf tPf2 in
-  let specReq = Requires (Unrefined, EApply (wp_X, eArgs @ [EVar s0; EVar wpContinue])) in
-  let specEns = Ensures (Unrefined, EApply (Id "eval_code", [eCode; EVar s0; EVar f0; EVar sM])) in
-  // wpProof_X body
-  //   let (sM, f0, g1, ..., gn) = va_lemma_X (va_code_X ARGS) s0 ARGS in
+  let specReq = Requires (Unrefined, EApply (wp_X, eArgs @ [EVar s0; EVar k_true])) in
+  let specEns = Ensures (Unrefined, eTrue) in
+  // wpCompute_X body
   let gAssigns = List.map (fun (x, _) -> (x, None)) ghostRets in
   let sCallLemma = SAssign ((sM, None)::(f0, None)::gAssigns, EApply (lemma_X, eCode::(EVar s0)::eArgs)) in
   let sAssignG = SAssign ([(g, None)], ghostRetTuple) in
+  let pCompute=
+    {
+      pname = wpCompute_X;
+      pghost = Ghost;
+      pinline = Outline;
+      pargs = pargs @ [pS0];
+      prets = [rSM; rF0; rG];
+      pspecs = [(loc, specReq); (loc, specEns)];
+      pbody = Some [sCallLemma; sAssignG];
+      pattrs = [(Id "reducible", [])];
+    }
+    in
+
+  // wpProof_X declaration
+  let pK = arg k tContinue in
+  let specEnsArgs = [eCode; appArgs wp_X; appArgs wpMonotone_X; appArgs wpCompute_X; EVar s0; EVar k] in
+  let specReq = Requires (Unrefined, EApply (wp_X, eArgs @ [EVar s0; EVar k])) in
+  let specEns = Ensures (Unrefined, EApply (Id "t_ensure", specEnsArgs)) in
+  // wpProof_X body
   let sLemmaUpd = SAssign ([], EApply (Reserved "lemma_upd_update", [EVar sM])) in
   let (_, eqUpdates) = Emit_common_lemmas.makeFrame env p s0 sM in
   let sAssertEq = SAssert (assert_attrs_default, eqUpdates) in
-  //   let f : (va_quickProc_q aN (qs sM) (wpContinue sM g) unit -> Ghost (state * fuel * aN) True (qs sM)) = fun x -> x () in
-  let tFRet = TApp (TName (Id "Ghost"), [tQsTuple; tTrue; tQ]) in
-  let tF = TApp (TName (Id "fun"), [tPf1; tFRet]) in
-  let eLambda = EBind (Lambda, [], [(x, None)], [], EApply (x, [eUnit])) in
-  let sAssignF = SAssign ([(f, Some (Some tF, Ghost))], eLambda) in
-  let sAssignPf = SAssign ([(pf, None)], EVar f) in
   let pProof =
     {
       pname = wpProof_X;
       pghost = Ghost;
       pinline = Outline;
-      pargs = pargs @ [pAN; pQs; pS0; pWpContinue];
-      prets = [rSM; rF0; rG; rPf];
+      pargs = pargs @ [pS0; pK];
+      prets = [];
       pspecs = [(loc, specReq); (loc, specEns)];
-      pbody = Some [sCallLemma; sAssignG; sLemmaUpd; sAssertEq; sAssignF; sAssignPf];
-      pattrs = [(Id "dependent", [])]
+      pbody = Some [sCallLemma; sLemmaUpd; sAssertEq];
+      pattrs = [];
     }
     in
+
   // quick_X
   //   va_QProc (va_code_X ARGS) (wp_X ARGS) (wpProof_X ARGS)
-  let applyOpt f args = match args with [] -> EVar f | _ -> EApply (f, args) in
-  let wpArgs = applyOpt wp_X eArgs in
-  let applyProof = applyOpt wpProof_X eArgs in
-  let eQuick = EApply (Reserved "QProc", [eCode; wpArgs; applyProof]) in
+  //   va_QProc (va_code_X ARGS) (wp_X ARGS) (wpMonotone_X ARGS) (wpCompute_X ARGS) (wpProof_X ARGS)
+  let tRetQuick = TApp (TName (Reserved "quickCode"), [tA; tCode]) in
+  let eQuick = EApply (Reserved "QProc", [eCode; appArgs wp_X; appArgs wpMonotone_X; appArgs wpCompute_X; appArgs wpProof_X]) in
   let fQuick =
     {
       fname = Reserved ("quick_" + (string_of_id p.pname));
@@ -217,4 +255,4 @@ let build_proc (env:env) (loc:loc) (p:proc_decl):decls =
       fattrs = [(Id "public", []); (Id "opaque_to_smt", [])];
     }
     in
-  [(loc, DFun fWp); (loc, DProc pProof); (loc, DFun fQuick)]
+  [(loc, DFun fWp); (loc, DProc pMonotone); (loc, DProc pCompute); (loc, DProc pProof); (loc, DFun fQuick)]
