src/arch/x64/X64.Vale.Quick_i.fst
@@ -1,50 +1,127 @@
 module X64.Vale.Quick_i
 
-let rec wp_sound #a cs fcs p s0 =
-  match fcs with
+let rec wp_monotone #a cs qcs k1 k2 s0 =
+  match qcs with
+  | QEmpty g -> ()
+  | QSeq qc qcs ->
+      let QProc _ wp1' monotone _ _ = qc in
+      let c::cs = cs in
+      let k1' = wp_Seq cs qcs k1 in
+      let k2' = wp_Seq cs qcs k2 in
+      let f s g : Lemma (k1' s g ==> k2' s g) =
+        wp_monotone cs qcs k1 k2 s
+        in
+      FStar.Classical.forall_intro_2 f;
+      assert (forall s g. k1' s g ==> k2' s g);
+      monotone s0 k1' k2'
+  | QBind qc qcs ->
+      let QProc c' wp1' monotone _ _ = qc in
+      let c::cs = cs in
+      let k1' = wp_Bind cs qcs k1 in
+      let k2' = wp_Bind cs qcs k2 in
+      let f s g : Lemma (k1' s g ==> k2' s g) =
+        wp_monotone cs (qcs g) k1 k2 s
+        in
+      FStar.Classical.forall_intro_2 f;
+      monotone s0 k1' k2'
+  | QGetState f ->
+      let c::cs = cs in
+      wp_monotone cs (f s0) k1 k2 s0
+  | QLemma pre post l qcs' ->
+      wp_monotone cs qcs' k1 k2 s0
+
+let rec wp_compute #a cs qcs s0 =
+  match qcs with
   | QEmpty g ->
       let (sN, fN) = va_lemma_empty_total s0 [] in (sN, fN, g)
-  | QSeq fc fcs ->
-      let QProc _ wp1' proof = fc in
+  | QSeq qc qcs ->
+      let QProc _ wp1' monotone compute proof = qc in
       let c::cs = cs in
-      let wp_continue = wp_Seq cs fcs p in
-      let qs (sM:state) ((sN:state), (fN:fuel), (gN:a)) : Type0 = eval (Block cs) sM fN sN /\ p sN gN in
-      let (|sM, fM, g1, pp|) = proof a qs s0 wp_continue in
-      let q = qs sM in
-      let proof_continue () : Ghost ((sN:state) * (fN:fuel) * (gN:a))
-        (requires wp_continue sM g1)
-        (ensures q) =
-        //assert (wp_continue sM g1);
-        //assert (wp cs fcs p sM);
-        wp_sound cs fcs p sM
-        in
-      let (sN, fN, gN) = pp proof_continue in
-      let fN' = va_lemma_merge_total (c::cs) s0 fM sM fN sN in
+      let k' = wp_Seq cs qcs k_true in
+      monotone s0 k' k_true;
+      let (sM, fM, gM) = compute s0 in
+      proof s0 k';
+      let (sN, fN, gN) = wp_compute cs qcs sM in
+      let fN' = va_compute_merge_total fM fN in
       (sN, fN', gN)
-  | QBind fc fcs ->
-      let QProc c' wp1' proof = fc in
+  | QBind qc qcs ->
+      let QProc c' wp1' monotone compute proof = qc in
       let c::cs = cs in
-      let wp_continue = wp_Bind cs fcs p in
-      let qs (sM:state) ((sN:state), (fN:fuel), (gN:a)) : Type0 = eval (Block cs) sM fN sN /\ p sN gN in
-      let (|sM, fM, g1, pp|) = proof a qs s0 wp_continue in
-      let q = qs sM in
-      let proof_continue () : Ghost ((sN:state) * (fN:fuel) * (gN:a))
-        (requires wp_continue sM g1)
-        (ensures q) =
-        //assert (wp_continue sM g1);
-        //assert (wp cs (fcs g1) p sM);
-        wp_sound cs (fcs g1) p sM
-        in
-      let (sN, fN, gN) = pp proof_continue in
-      let fN' = va_lemma_merge_total (c::cs) s0 fM sM fN sN in
+      let k' = wp_Bind cs qcs k_true in
+      monotone s0 k' k_true;
+      let (sM, fM, gM) = compute s0 in
+      proof s0 k';
+      let (sN, fN, gN) = wp_compute cs (qcs gM) sM in
+      let fN' = va_compute_merge_total fM fN in
       (sN, fN', gN)
   | QGetState f ->
       let c::cs = cs in
       let (sM, fM) = va_lemma_empty_total s0 [] in
-      let (sN, fN, gN) = wp_sound cs (f sM) p sM in
-      let fN' = va_lemma_merge_total (c::cs) s0 fM sM fN sN in
+      let (sN, fN, gN) = wp_compute cs (f sM) sM in
+      let fN' = va_compute_merge_total fM fN in
       (sN, fN', gN)
-  | QLemma pre post l fcs' ->
-      let _ = FStar.Classical.arrow_to_impl #pre #post l in
-      wp_sound cs fcs' p s0
+  | QLemma pre post l qcs' ->
+      l ();
+      wp_compute cs qcs' s0
+
+let rec wp_sound #a cs qcs k s0 =
+  match qcs with
+  | QEmpty g ->
+      let (sN, fN) = va_lemma_empty_total s0 [] in ()
+  | QSeq qc qcs ->
+      let QProc _ wp1' monotone compute proof = qc in
+      let c::cs = cs in
+      let k' = wp_Seq cs qcs k in
+      monotone s0 k' k_true;
+      let (sM, fM, gM) = compute s0 in
+      proof s0 k';
+      wp_monotone cs qcs k k_true sM;
+      let (sN, fN, gN) = wp_compute cs qcs sM in
+      wp_sound cs qcs k sM;
+      let fN' = va_lemma_merge_total (c::cs) s0 fM sM fN sN in
+      ()
+  | QBind qc qcs ->
+      let QProc c' wp1' monotone compute proof = qc in
+      let c::cs = cs in
+      let k' = wp_Bind cs qcs k in
+      monotone s0 k' k_true;
+      let (sM, fM, gM) = compute s0 in
+      proof s0 k';
+      wp_monotone cs (qcs gM) k k_true sM;
+      let (sN, fN, gN) = wp_compute cs (qcs gM) sM in
+      wp_sound cs (qcs gM) k sM;
+      let fN' = va_lemma_merge_total (c::cs) s0 fM sM fN sN in
+      ()
+  | QGetState f ->
+      let c::cs = cs in
+      let (sM, fM) = va_lemma_empty_total s0 [] in
+      wp_sound cs (f sM) k sM;
+      wp_monotone cs (f sM) k k_true sM;
+      let (sN, fN, gN) = wp_compute cs (f sM) sM in
+      let fN' = va_lemma_merge_total (c::cs) s0 fM sM fN sN in
+      ()
+  | QLemma pre post l qcs' ->
+      l ();
+      wp_sound cs qcs' k s0
+
+let qblock_monotone #a #cs qcs s0 k1 k2 =
+  wp_monotone cs qcs k1 k2 s0
+
+let qblock_compute #a #cs qcs s0 =
+  wp_compute cs qcs s0
+
+let qblock_proof #a #cs qcs s0 k =
+  wp_monotone cs qcs k k_true s0;
+  let (sM, f0, g) = wp_compute cs qcs s0 in
+  wp_sound cs qcs k s0
+
+let wp_sound_code #a c qc k s0 =
+  let QProc c wp monotone compute proof = qc in
+  monotone s0 k k_true;
+  let (sM, f0, g) = compute s0 in
+  proof s0 k;
+  (sM, f0, g)
+
+let wp_sound_wrap #a cs qcs s0 k = wp_sound cs qcs (k s0) s0; wp_monotone cs qcs (k s0) k_true s0; wp_compute cs qcs s0
+let wp_sound_code_wrap #a c qc s0 k = wp_sound_code c qc (k s0) s0
 
