src/arch/x64/X64.Vale.Quick_i.fsti
@@ -11,54 +11,85 @@ unfold let fuel = va_fuel
 unfold let eval = eval_code
 let if_codes (b:bool) (cs1:codes) (cs2:codes) : codes = if b then cs1 else cs2
 
-let lemma (pre:Type0) (post:Type0) : Type0 =
-  squash pre -> GTot (squash post)
-
 noeq type quickCodes (a:Type0) : codes -> Type =
 | QEmpty: a -> quickCodes a []
 | QSeq: #b:Type -> #c:code -> #cs:codes -> quickCode b c -> quickCodes a cs -> quickCodes a (c::cs)
 | QBind: #b:Type -> #c:code -> #cs:codes -> quickCode b c -> (b -> quickCodes a cs) -> quickCodes a (c::cs)
 | QGetState: #cs:codes -> (state -> quickCodes a cs) -> quickCodes a ((Block [])::cs)
-| QLemma: #cs:codes -> pre:Type0 -> post:Type0 -> lemma pre post -> quickCodes a cs -> quickCodes a cs
+| QLemma: #cs:codes -> pre:Type0 -> post:Type0 -> (unit -> Lemma (requires pre) (ensures post)) -> quickCodes a cs -> quickCodes a cs
 
-let wpLemma (#cs:codes) (#pre:Type0) (#post:Type0) (#a:Type0) (l:lemma pre post) (fcs:quickCodes a cs) : quickCodes a cs =
-  QLemma pre post l fcs
+let wpLemma (#cs:codes) (#pre:Type0) (#post:Type0) (#a:Type0) ($l:unit -> Lemma (requires pre) (ensures post)) (qcs:quickCodes a cs) : quickCodes a cs =
+  QLemma pre post l qcs
 
-let wp_proc (#a:Type0) (c:code) (fc:quickCode a c) (s0:state) (wp_continue:state -> a -> Type0) : Type0 =
-  match fc with
-  | QProc _ wp1' _ -> wp1' s0 wp_continue
+let wp_proc (#a:Type0) (c:code) (qc:quickCode a c) (s0:state) (k:state -> a -> Type0) : Type0 =
+  match qc with
+  | QProc _ wp _ _ _ -> wp s0 k
 
 let wp_Seq_t (a:Type0) = state -> a -> Type0
 let wp_Bind_t (a:Type0) = state -> a -> Type0
-let rec wp (#a:Type0) (cs:codes) (fcs:quickCodes a cs) (p:state -> a -> Type0) (s0:state) :
-  Tot Type0 (decreases %[cs; 0; fcs])
+let rec wp (#a:Type0) (cs:codes) (qcs:quickCodes a cs) (k:state -> a -> Type0) (s0:state) :
+  Tot Type0 (decreases %[cs; 0; qcs])
   =
-  match fcs with
-  | QEmpty g -> p s0 g
-  | QSeq fc fcs ->
+  match qcs with
+  | QEmpty g -> k s0 g
+  | QSeq qc qcs ->
       let c::cs = cs in
-      wp_proc c fc s0 (wp_Seq cs fcs p)
-  | QBind fc fcs ->
+      wp_proc c qc s0 (wp_Seq cs qcs k)
+  | QBind qc qcs ->
       let c::cs = cs in
-      wp_proc c fc s0 (wp_Bind cs fcs p)
+      wp_proc c qc s0 (wp_Bind cs qcs k)
   | QGetState f ->
       let c::cs = cs in
-      wp cs (f s0) p s0
-  | QLemma pre post l fcs -> pre /\ (post ==> wp cs fcs p s0)
+      wp cs (f s0) k s0
+  | QLemma pre post l qcs -> pre /\ (post ==> wp cs qcs k s0)
 // Hoist lambdas out of main definition to avoid issues with function equality 
-and wp_Seq (#a:Type0) (#b:Type0) (cs:codes) (fcs:quickCodes b cs) (p:state -> b -> Type0) :
-  Tot (wp_Seq_t a) (decreases %[cs; 1; fcs])
+and wp_Seq (#a:Type0) (#b:Type0) (cs:codes) (qcs:quickCodes b cs) (k:state -> b -> Type0) :
+  Tot (wp_Seq_t a) (decreases %[cs; 1; qcs])
   =
-  let f s0 _ = wp cs fcs p s0 in f
-and wp_Bind (#a:Type0) (#b:Type0) (cs:codes) (fcs:a -> quickCodes b cs) (p:state -> b -> Type0) :
-  Tot (wp_Bind_t a) (decreases %[cs; 1; fcs])
+  let f s0 _ = wp cs qcs k s0 in f
+and wp_Bind (#a:Type0) (#b:Type0) (cs:codes) (qcs:a -> quickCodes b cs) (k:state -> b -> Type0) :
+  Tot (wp_Bind_t a) (decreases %[cs; 1; qcs])
   =
-  let f s0 g = wp cs (fcs g) p s0 in f
+  let f s0 g = wp cs (qcs g) k s0 in f
 
-val wp_sound (#a:Type0) (cs:codes) (fcs:quickCodes a cs) (p:state -> a -> Type0) (s0:state) :
+val wp_monotone (#a:Type0) (cs:codes) (qcs:quickCodes a cs) (k1:state -> a -> Type0) (k2:state -> a -> Type0) (s0:state) : Lemma
+  (requires (forall (s:state) (g:a). k1 s g ==> k2 s g))
+  (ensures wp cs qcs k1 s0 ==> wp cs qcs k2 s0)
+
+val wp_compute (#a:Type0) (cs:codes) (qcs:quickCodes a cs) (s0:state) :
   Ghost ((sN:state) * (fN:fuel) * (g:a))
-  (requires wp cs fcs p s0)
-  (ensures fun (sN, fN, gN) -> eval (Block cs) s0 fN sN /\ p sN gN)
+  (requires wp cs qcs k_true s0)
+  (ensures fun _ -> True)
+
+val wp_sound (#a:Type0) (cs:codes) (qcs:quickCodes a cs) (k:state -> a -> Type0) (s0:state) : Lemma
+  (requires wp cs qcs k s0)
+  (ensures (wp_monotone cs qcs k k_true s0; let (sN, fN, gN) = wp_compute cs qcs s0 in eval (Block cs) s0 fN sN /\ k sN gN))
+
+unfold let block = va_Block
+
+let wp_block (#a:Type) (#cs:codes) (qcs:quickCodes a cs) (s0:state) (k:state -> a -> Type0) : Type0 =
+  wp cs qcs k s0
+
+val qblock_monotone (#a:Type) (#cs:codes) (qcs:quickCodes a cs) (s0:state) (k1:state -> a -> Type0) (k2:state -> a -> Type0) : Lemma
+  (requires (forall (s:state) (g:a). k1 s g ==> k2 s g))
+  (ensures wp_block qcs s0 k1 ==> wp_block qcs s0 k2)
+
+val qblock_compute (#a:Type) (#cs:codes) (qcs:quickCodes a cs) (s0:state) : Ghost (state * fuel * a)
+  (requires wp_block qcs s0 k_true)
+  (ensures fun _ -> True)
+
+val qblock_proof (#a:Type) (#cs:codes) (qcs:quickCodes a cs) (s0:state) (k:state -> a -> Type0) : Lemma
+  (requires wp_block qcs s0 k)
+  (ensures (qblock_monotone qcs s0 k k_true; let (sM, f0, g) = qblock_compute qcs s0 in eval_code (block cs) s0 f0 sM /\ k sM g))
+
+[@"opaque_to_smt"]
+let qblock (#a:Type) (#cs:codes) (qcs:quickCodes a cs) : quickCode a (block cs) =
+  QProc (block cs) (wp_block qcs) (qblock_monotone qcs) (qblock_compute qcs) (qblock_proof qcs)
+
+val wp_sound_code (#a:Type0) (c:code) (qc:quickCode a c) (k:state -> a -> Type0) (s0:state) :
+  Ghost ((sN:state) * (fN:fuel) * (g:a))
+  (requires QProc?.wp qc s0 k)
+  (ensures fun (sN, fN, gN) -> eval_code c s0 fN sN /\ k sN gN)
 
 let rec regs_match (regs:list reg) (r0:Regs_i.t) (r1:Regs_i.t) : Type0 =
   match regs with
@@ -70,7 +101,7 @@ let all_regs_match (r0:Regs_i.t) (r1:Regs_i.t) : Type0
   let regs = [Rax; Rbx; Rcx; Rdx; Rsi; Rdi; Rbp; Rsp; R8; R9; R10; R11; R12; R13; R14; R15] in
   regs_match regs r0 r1
 
-let state_match (s0:state) (s1:state) : Pure Type0
+let va_state_match (s0:state) (s1:state) : Pure Type0
   (requires True)
   (ensures fun b -> b ==> state_eq s0 s1)
   =
@@ -80,16 +111,48 @@ let state_match (s0:state) (s1:state) : Pure Type0
   s0.flags == s1.flags /\
   s0.mem == s1.mem
 
+unfold let wp_sound_pre (#a:Type0) (#cs:codes) (qcs:quickCodes a cs) (s0:state) (k:state -> state -> a -> Type0) : Type0 =
+  forall (ok:bool) (regs:Regs_i.t) (flags:nat64) (mem:mem).
+    let s0' = {ok = ok; regs = regs; flags = flags; mem = mem} in
+    s0 == s0' ==> wp cs qcs (k s0') s0'
+
+unfold let wp_sound_post (#a:Type0) (#cs:codes) (qcs:quickCodes a cs) (s0:state) (k:state -> state -> a -> Type0) ((sN:state), (fN:fuel), (gN:a)) : Type0 =
+  eval (Block cs) s0 fN sN /\
+  k s0 sN gN
+
+val wp_sound_wrap (#a:Type0) (cs:codes) (qcs:quickCodes a cs) (s0:state) (k:state -> state -> a -> Type0) :
+  Ghost (state * fuel * a)
+    (wp_sound_pre qcs s0 k)
+    (wp_sound_post qcs s0 k)
+
+unfold let wp_sound_code_pre (#a:Type0) (#c:code) (qc:quickCode a c) (s0:state) (k:state -> state -> a -> Type0) : Type0 =
+  forall (ok:bool) (regs:Regs_i.t) (flags:nat64) (mem:mem).
+    let s0' = {ok = ok; regs = regs; flags = flags; mem = mem} in
+    s0 == s0' ==> QProc?.wp qc s0' (k s0')
+
+unfold let wp_sound_code_post (#a:Type0) (#c:code) (qc:quickCode a c) (s0:state) (k:state -> state -> a -> Type0) ((sN:state), (fN:fuel), (gN:a)) : Type0 =
+  eval c s0 fN sN /\
+  k s0 sN gN
+
+val wp_sound_code_wrap (#a:Type0) (c:code) (qc:quickCode a c) (s0:state) (k:state -> state -> a -> Type0) :
+  Ghost (state * fuel * a)
+    (wp_sound_code_pre qc s0 k)
+    (wp_sound_code_post qc s0 k)
+
 unfold let normal_steps : list string =
   [
     "X64.Vale.Quick_i.wp";
     "X64.Vale.Quick_i.wp_proc";
     "X64.Vale.Quick_i.wp_Seq";
     "X64.Vale.Quick_i.wp_Bind";
+    "X64.Vale.Quick_i.wp_block";
+    "X64.Vale.Quick_i.qblock";
     "X64.Vale.Quick_i.wpLemma";
     "X64.Vale.Quick_i.regs_match";
     "X64.Vale.Quick_i.all_regs_match";
-    "X64.Vale.Quick_i.state_match";
+    "X64.Vale.Quick_i.va_state_match";
+    "X64.Vale.Quick_i.wp_sound_pre";
+    "X64.Vale.Quick_i.wp_sound_code_pre";
 
     "X64.Machine_s.__proj__OReg__item__r";
     "X64.Machine_s.uu___is_OReg";
@@ -107,6 +170,7 @@ unfold let normal_steps : list string =
     "X64.Vale.State_i.state_eq";
 
     "X64.Vale.Decls.va_QProc";
+    "X64.Vale.Decls.__proj__QProc__item__wp";
     "X64.Vale.Decls.va_eval_dst_opr64";
     "X64.Vale.Decls.va_eval_opr64";
     "X64.Vale.Decls.va_is_dst_opr64";
@@ -117,7 +181,7 @@ unfold let normal_steps : list string =
     "X64.Vale.Decls.va_get_flags";
     "X64.Vale.Decls.va_get_mem";
     "X64.Vale.Decls.va_get_reg";
-    "X64.Vale.Decls.va_update_reg";
+    "X64.Vale.Decls.va_update_ok";
     "X64.Vale.Decls.va_update_flags";
     "X64.Vale.Decls.va_update_mem";
     "X64.Vale.Decls.va_update_reg";
@@ -125,5 +189,9 @@ unfold let normal_steps : list string =
     "X64.Vale.Decls.va_upd_flags";
     "X64.Vale.Decls.va_upd_mem";
     "X64.Vale.Decls.va_upd_operand_dst_opr64";
+    "X64.Vale.Decls.va_CCons";
+    "X64.Vale.Decls.va_CNil";
+    "X64.Vale.Decls.va_op_dst_opr64_reg";
+    "X64.Vale.Decls.va_const_opr64";
   ]
 
